TypeProperties.v
@@ -8,5 +8,4 @@ From Elo Require Export SafeNewX.
 From Elo Require Export SafeAcq.
 From Elo Require Export SafeCR.
 From Elo Require Export SafeSpawns.
-From Elo Require Export ConsistentRegions.
 
